WIP election

examples/Messaging/Election.v
@@ -8,7 +8,8 @@ From Coq Require Import
      Lia
      Vector
      List
-     Arith.PeanoNat.
+     Arith.PeanoNat
+     Wellfounded Relations.Relation_Operators.
 
 From ITree Require Import
      CategoryOps.
@@ -27,53 +28,12 @@ From CTree Require Import
      Logic.Ctl
      Misc.Vectors.
 
-From Equations Require Import Equations.
-
 Import CTreeNotations ListNotations VectorNotations CtlNotations.
 Local Open Scope vector_scope.
 Local Open Scope ctree_scope.
 Local Open Scope ctl_scope.
 
 Set Implicit Arguments.
-
-Variant message :=
-  | Candidate (u: nat)
-  | Elected (u: nat).
-
-Definition proc_handle_msg (id: uid)(right: uid) (m: option message): ctree (netE message) B01 (unit + unit) :=
-       match m with
-       | Some (Candidate candidate) =>
-           match Nat.compare candidate id with (* candidate < id *)
-           (* My [left] neighbor proposed a candidate, I support that candidate *)
-           | Gt => send id right (Candidate candidate) ;; Ret (inl tt)
-           (* My left neighbor proposed a candidate, I do not support him *)
-           | Lt => Ret (inl tt)
-           (* I am the leader, but only I know *)
-           | Datatypes.Eq => send id right (Elected id) ;; Ret (inr tt)
-           end
-       | Some (Elected x) =>
-           (* I know [x] is the leader *)
-           send id right (Elected x) ;; Ret (inr tt)
-       | None => Ret (inl tt) (* Didn't receive anything *)
-       end.
-
-Definition proc_loop (id: uid)(right: uid): ctree (netE message) B01 unit :=
-  CTree.iter
-    (fun _ =>
-       m <- recv id;;
-       proc_handle_msg id right m) tt.
-
-(* send from to msg *)
-(* Before: Switch_to i ~> event modelling that process i is being scheduled
-   This is currently removed
- *)
-(*| Client process |*)
-Definition proc (id: uid)(n: nat): ctree (netE message) B01 unit :=
-  let right := modulo (S id) n in
-  (* 1. Send my [id] to the process on the right *)
-  send id right (Candidate id);;
-  (* 2. Loop until we know the leader *)
-  proc_loop id right.
 
 (*
   For the system "sched {proc(id,n) | 0 <= id < n}"
@@ -133,25 +93,44 @@ V ==> AF (sched n proc) |- V décroit strict
 
 Section Fair.
   Context {E C : Type -> Type} {X : Type} `{HasB0: B0 -< C} (n : nat).
+
+  (* FIXME the scheduler should have some kind of state *)
   Variable sched : vec n (ctree E C X) -> ctree E C X.
+  Variable next_id : vec n (ctree E C X) -> fin n.
 
   (* Transitions of the scheduled ctree are necessarily taken from
      the individual processes *)
-  Definition sched_correct := forall v l T',
-    trans l (sched v) T' ->
-    exists (i : fin n) t',
-    trans l (Vector.nth v i) t' /\ T' ≅ sched (replace v i t').
+  (* FIXME Ret *)
+  Definition sched_correct :=
+    forall v,
+    (* the scheduling can only be stuck if all the processes are stuck *)
+    (forall i l t', trans l v[@i] t' -> exists l' t'', trans l' v[@next_id v] t'') /\
+    (* all the transitions of the next scheduled process appear in the scheduled ctrees *)
+    (forall l t', trans l v[@next_id v] t' -> trans l (sched v) (sched (replace v (next_id v) t'))) /\
+    (* and no other transitions are possible *)
+    forall l T', trans l (sched v) T' -> exists t', trans l v[@next_id v] t' /\ T' ≅ sched (replace v (next_id v) t').
+
+  Lemma sched_correct_ktrans : sched_correct ->
+    forall S h v,
+    (forall i t' st st', ktrans (S := S) (h := h) (v[@i], st) (t', st') -> exists t'' st'', ktrans (S := S) (h := h) (v[@next_id v], st) (t'', st'')) /\
+    (forall T' st st',
+      ktrans (S := S) (h := h) (sched v, st) (T', st') ->
+      exists t',
+      ktrans (Vector.nth v (next_id v), st) (t', st') /\ T' ≅ sched (replace v (next_id v) t')) /\
+    (forall t' st st',
+      ktrans (S := S) (h := h) (v[@next_id v], st) (t', st') ->
+      ktrans (S := S) (h := h) (sched v, st) (sched (replace v (next_id v) t'), st')).
+  Admitted.
 
   (* Process i will make some progress in finite time
      sched_fair1_ i v ≜ eventually, sched (v1,..,vn) ~>* sched (v1', ..vi, ..,vn') ~> sched (v1', ..vi',..,vn')
    *)
   Inductive sched_fair1_ i : vec n (ctree E C X) -> Prop :=
   | sched_fair1_now : forall v,
-    (forall l t', trans l v[@i] t' -> trans l (sched v) (sched (replace v i t'))) ->
-    (forall l T', trans l (sched v) T' -> exists t', trans l v[@i] t' /\ T' ≅ (sched (replace v i t'))) ->
+    next_id v = i ->
     sched_fair1_ i v
   | sched_fair1_later : forall v,
-    (exists l T', trans l (sched v) T') /\
+    next_id v <> i ->
     (forall l v',
       trans l (sched v) (sched v') ->
       sched_fair1_ i v') ->
@@ -170,15 +149,19 @@ Section Fair.
   (* Whenever a process can progress, it will do so in finite time *)
   Definition sched_fair := forall v, (gfp sched_fairF) v.
 
-  Lemma sched_fair_not_stuck : sched_correct -> sched_fair -> forall v i, ~ is_stuck v[@i] -> ~ is_stuck (sched v).
+  Lemma sched_fair_not_stuck : sched_correct -> forall v i, ~ is_stuck v[@i] -> ~ is_stuck (sched v).
   Proof.
-    intros.
-    red in H0. specialize (H0 v). step in H0. destruct H0.
-    intro. apply H1. red. intros. intro.
-    apply H0 in H4 as ?. destruct H5.
-    - apply H5 in H4. now apply H3 in H4.
-    - destruct (H5) as [(? & ? & ?) _]. now apply H3 in H6.
+    intros. intro. apply H0. red. intros. intro.
+    apply H in H2 as (? & ? & ?).
+    apply H in H2. now apply H1 in H2.
   Qed.
+
+  Record FairSched := {
+    fsched : vec n (ctree E C X) -> ctree E C X;
+    fnext_id : vec n (ctree E C X) -> fin n;
+    fsched_correct : sched_correct;
+    fsched_fair : sched_fair;
+  }.
 
   (* What happens if
      [vi] : [Ret v -val v> ∅]
@@ -194,58 +177,52 @@ Proof.
   intros. inversion H0; subst; etrans.
 Qed.
 
-(* Attempt to have a meta-theorem reducing the correctness and termination of a "scheduled" system *)
-Theorem distr_system_dec_variant : forall {n C X St Msg} `{HasB0: B0 -< C}
+(* Meta-theorem reducing the correctness and termination of a "scheduled" system *)
+Theorem distr_system_dec_variant : forall {n C X St Msg V } `{HasB0: B0 -< C}
   (h : list (list Msg) -> St -> forall X, netE Msg X -> St)
+  (sched : vec n (ctree (netE Msg) C X) -> ctree (netE Msg) C X) next_id
+  (Hc : sched_correct sched next_id)
   (Inv : vec n (ctree (netE Msg) C X) -> list (list Msg) -> St -> Prop)
-  (var : St -> nat)
+  (var : St -> V) (v0 : V) i k φ
   (Hprog :
-    forall (sched : vec n (ctree (netE Msg) C X) -> ctree (netE Msg) C X)
-    (Hc : sched_correct sched) (*(Hf : sched_fair (HasB0 := HasB0) sched)*)
-    v qs st, Inv v qs st -> var st > 0 -> ~is_stuck (sched v))
+    forall v qs st, Inv v qs st -> var st <> v0 -> exists l T', trans l (sched v) T')
+  (Hinv :
+    forall v st st' qs qs' k t',
+    Inv v qs st ->
+    ktrans (h := handler_netE h) (v[@k], (qs, st)) (t', (qs', st')) ->
+    Inv (replace v k t') qs' st')
   (Hdec :
-    forall (sched : vec n (ctree (netE Msg) C X) -> ctree (netE Msg) C X)
-    (Hc : sched_correct sched) (*(Hf : sched_fair (HasB0 := HasB0) sched)*)
-    v qs st, Inv v qs st -> var st > 0 ->
-    forall v' qs' st', ktrans (h := handler_netE h) (sched v, (qs, st)) (sched v', (qs', st')) ->
-    Inv v' qs' st' /\ var st' < var st),
-  forall (sched : vec n (ctree (netE Msg) C X) -> ctree (netE Msg) C X)
-  (Hc : sched_correct sched) (*(Hf : sched_fair (HasB0 := HasB0) sched)*) v qs st,
+    forall v qs st,
+    Inv v qs st ->
+    var st = i ->
+    next_id v = k ->
+    entailsF (h := handler_netE h) <(AF φ)> (sched v) (qs, st))
+  (Hcst :
+    forall v T st st' qs qs',
+    Inv v qs st ->
+    var st = i ->
+    next_id v <> k ->
+    ktrans (h := handler_netE h) (sched v, (qs, st)) (T, (qs', st')) -> var st' = i),
+  forall (Hf : sched_fair (HasB0 := HasB0) sched next_id) v qs st,
   Inv v qs st ->
-  (* Then the global system reaches *)
-  entailsF (h := handler_netE h) <(AF (now {(fun '(qs, st) => var st = 0)}))> (sched v) (qs, st).
+  var st = i ->
+  i <> v0 ->
+  entailsF (h := handler_netE h) <(AF φ)> (sched v) (qs, st).
 Proof.
   intros.
-  remember (var st) as i. assert (var st <= i)%nat by lia. clear Heqi.
-  revert v qs st H H0. induction i; intros.
-  - left. cbn. lia.
-  - inversion H0. 2: { apply IHi; auto. }
-    next. right. apply ctl_ax. intros. apply ktrans_trans in H1 as ?.
-    destruct (H3) as [ [] | (? & ? & ? & ?) ]; clear H3.
-    + apply Hc in H4 as (? & ? & ? & ?).
-      rewrite H4 in H1.
-      cbn in Hdec. destruct s'.
-      unshelve epose proof (Hdec _ _ _ _ _ _ _ _ _ _ H1) as []; auto.
-      lia.
-      assert (var s <= i)%nat by lia.
-      replace t' with (sched (replace v x0 x1)) by admit.
-      apply IHi; auto.
-    + subst. exfalso. subs.
+  specialize (Hf v). step in Hf. destruct Hf. clear H3. red in H2.
+  clear H2. assert (H2 : sched_fair1_ sched next_id k v) by admit.
+  revert qs st H H0.
+  induction H2; intros.
+  - now eapply Hdec.
+  - next. right. apply ctl_ax. intros.
+    apply ktrans_trans in H5 as ?. destruct H6; [| admit].
+    destruct H6. destruct s'.
+    destruct (Hc v) as (? & _ & ?). specialize (H8 x t' H6). destruct H8 as (? & ? & ?). subs.
+    eapply H2; eauto. eapply Hinv; eauto. admit.
 Admitted.
 
-(* Logical state: the logical information about the dynamics we wish to keep track of. *)
-Variant candidate_state : Type :=
-| CandBegin
-| CandTraveling (d: nat)
-| CandLost.
-
-Variant election_state : Type :=
-(* First phase of the protocol *)
-| VCandidates (l: list candidate_state)
-(* Second phase of the protocol *)
-| VElected (i: nat) (* i => i hops *)
-.
-
+(* TODO clean up, use more section variables *)
 Definition ids_wf {n} (ids : vec n nat) :=
   forall j k, j <> k -> Vector.nth ids j <> Vector.nth ids k.
 
@@ -259,6 +236,87 @@ Admitted.
 Section Election.
 
 Context {n : nat} (Hn : n <> 0) (ids : vec n nat) (wf : ids_wf ids).
+
+Variant message :=
+  | Candidate (u: nat)
+  | Elected (u: nat).
+
+(* TODO use ids *)
+Definition proc_handle_msg (id: uid)(right: uid) (m: option message): ctree (netE message) B01 (unit + unit) :=
+       match m with
+       | Some (Candidate candidate) =>
+           match Nat.compare candidate id with (* candidate < id *)
+           (* My [left] neighbor proposed a candidate, I support that candidate *)
+           | Gt => send id right (Candidate candidate) ;; Ret (inl tt)
+           (* My left neighbor proposed a candidate, I do not support him *)
+           | Lt => Ret (inl tt)
+           (* I am the leader, but only I know *)
+           | Datatypes.Eq => send id right (Elected id) ;; Ret (inr tt)
+           end
+       | Some (Elected x) =>
+           (* I know [x] is the leader *)
+           send id right (Elected x) ;; Ret (inr tt)
+       | None => Ret (inl tt) (* Didn't receive anything *)
+       end.
+
+Definition proc_loop (id: uid)(right: uid): ctree (netE message) B01 unit :=
+  CTree.iter
+    (fun _ =>
+       m <- recv id;;
+       proc_handle_msg id right m) tt.
+
+Definition proc_loop_handle_msg (id: uid)(right: uid) (m: option message): ctree (netE message) B01 unit :=
+  lr <- proc_handle_msg id right m;;
+  match lr with
+  | inl l => Guard (proc_loop id right)
+  | inr r => Ret r
+  end.
+
+(* send from to msg *)
+(* Before: Switch_to i ~> event modelling that process i is being scheduled
+   This is currently removed
+ *)
+(*| Client process |*)
+Definition proc (id: uid)(right: nat): ctree (netE message) B01 unit :=
+  (* 1. Send my [id] to the process on the right *)
+  send id right (Candidate id);;
+  (* 2. Loop until we know the leader *)
+  proc_loop id right.
+
+(* Logical state: the logical information about the dynamics we wish to keep track of. *)
+Variant proc_state : Type :=
+| ProcBegin
+| ProcWaiting
+| ProcProcessing (m: message)
+| ProcElected.
+
+Variant election_progress :=
+| MaxCandidate (n : nat)
+| MaxElected (n : nat).
+
+Record election_state : Type := mk_election_state {
+  s_procs : list proc_state;
+  (* Distance traveled by the max candidate message, or by the elected message *)
+  s_progress : election_progress;
+  (* Messages before proccesing the next message that will make the system progress,
+     and whether the first message in the queue is being processed *)
+  s_queue : nat * bool;
+}.
+
+(* The extended mailbox of a process is its mailbox
+   plus the message it's currently processing, if any *)
+Definition ext_mailbox1 '(q, p) :=
+  match p with
+  | ProcProcessing p => (p::q)%list
+  | _ => q
+  end.
+
+Definition ext_mailbox qs st :=
+  List.map ext_mailbox1 (combine qs st.(s_procs)).
+
+Context (sched : vec n (ctree (netE message) B01 unit) -> ctree (netE message) B01 unit).
+Context (next_id : vec n (ctree (netE message) B01 unit) -> fin n).
+Context (Hc : sched_correct sched next_id).
 
 Open Scope nat_scope.
 
@@ -276,139 +334,419 @@ Proof.
   intros. destruct H. unfold from_to_ in *. lia.
 Qed.
 
-Definition fin_of_nat_mod i : fin n :=
-  Fin.of_nat_lt (p := i mod n) (Nat.mod_upper_bound i n Hn).
+Lemma from_to__dec : forall (i j k : nat), { from_to_ i j k } + { ~from_to_ i j k }.
+Proof.
+  intros. unfold from_to_.
+  destruct (Compare_dec.le_dec i k).
+  2: tauto.
+  destruct (Compare_dec.lt_dec k j); tauto.
+Qed.
 
-(* Invariant during phase 1 (Candidate messages)
-   Three components in the "moral" configuration: the code, the dynamic state, the logical state
- *)
-Definition election_invariant_candidates
-  (cand_progress : list candidate_state) qs :=
-  (* Well-formedness *)
-  List.length cand_progress = n /\
-  List.nth (proj1_sig (Fin.to_nat (max_id wf))) cand_progress CandLost <> CandLost /\
-  forall i (Hi : (i < n)%nat),
-    (List.nth_error cand_progress i = Some CandBegin \/ List.nth_error cand_progress i = Some CandLost) ->
-      ~ In (Candidate i) (concat qs) /\
-    forall p, List.nth_error cand_progress i = Some (CandTraveling p) ->
-      let i' := Fin.of_nat_lt Hi in
-      let s := (i + 1) mod n in
-      let j := (i + p + 1) mod n in
-      (In (Candidate n) (List.nth j qs []%list)) /\
-      (forall k (Hk: from_to s j k),
-        let k' := Fin.of_nat_lt (@from_to_bound s j k (Nat.mod_upper_bound _ _ Hn) (Nat.mod_upper_bound _ _ Hn) Hk) in
-        Vector.nth ids k' < Vector.nth ids i' /\
-        (i' = max_id wf -> k <> i -> List.nth_error cand_progress k = Some CandLost)).
+Lemma from_to_dec : forall (i j k : nat), { from_to i j k } + { ~from_to i j k }.
+Proof.
+  intros. unfold from_to. Locate "<=". Search nat le sumbool.
+  destruct (Compare_dec.le_lt_dec i j).
+  - destruct (from_to__dec i j k); [| tauto].
+    left. split; [tauto | lia].
+  - destruct (from_to__dec j n k); [| tauto].
+    destruct (from_to__dec 0 i k); [| tauto].
+    left. split; [lia | tauto].
+Qed.
 
-(* Invariant during phase 2 (Elected message) *)
-Definition election_invariant_elected
-  (elected_progress : nat) (qs: list (list message)) :=
-  forall (He : elected_progress < n),
-  let m := proj1_sig (Fin.to_nat (max_id wf)) in
-  let e' := Fin.of_nat_lt He in
-  let j := (m + elected_progress + 1) mod n in
-  List.nth j qs []%list = [Elected m]%list /\
-  forall k, k <> j -> List.nth k qs []%list = []%list.
-
-Definition election_state_invariant st qs :=
-  match st with
-  | VCandidates l => election_invariant_candidates l qs
-  | VElected n => election_invariant_elected n qs
+Definition next_proc_and_msg st :=
+  let m := (proj1_sig (Fin.to_nat (max_id wf))) in
+  match st.(s_progress) with
+  | MaxCandidate d => ((m + d) mod n, Candidate m)
+  | MaxElected d => ((m + d + 1) mod n, Elected m)
   end.
 
-Definition election_src_invariant_candidate st i (t : ctree (netE message) B01 unit) :=
-  match st with
-  | CandBegin => t ≅ proc i n
-  | CandTraveling j =>
-    (j < n -> t ≅ proc_loop i ((i + 1) mod n)) /\
-    (j = n -> t ≅ Ret tt)
-  | CandLost => t ≅ proc_loop i ((i + 1) mod n)
+Definition next_proc st :=
+  fst (next_proc_and_msg st).
+
+Definition handle_recv (q : nat * bool) :=
+  (if snd q then fst q - 1 else fst q, true).
+
+Definition handle_next qs st i :=
+  let l := List.length (List.nth i (ext_mailbox qs st) []%list) in
+  match List.nth i st.(s_procs) ProcBegin with
+  | ProcBegin => (l + 1, true)
+  | ProcProcessing _ => (l, true)
+  | _ => (l, false)
   end.
 
-Definition election_src_invariant st (v : vec n (ctree (netE message) B01 unit)) :=
-  match st with
-  | VCandidates l => forall i (Hi : i < n),
-    election_src_invariant_candidate (nth i l CandLost) i v[@Fin.of_nat_lt Hi]
-  | VElected d =>
-    let m := proj1_sig (Fin.to_nat (max_id wf)) in
-    forall i (Hi: i < n),
-    (from_to ((S m) mod n) ((m + d + 1) mod n) i ->
-      v[@Fin.of_nat_lt Hi] ≅ Ret tt) /\
-    (not (from_to ((S m) mod n) ((m + d + 1) mod n) i) ->
-      v[@Fin.of_nat_lt Hi] ≅ proc_loop i ((i + 1) mod n))
-  end.
-
-Definition election_invariant v qs st := election_state_invariant st qs /\ election_src_invariant st v.
-
-Definition cand_state_value (st : candidate_state) :=
-  match st with
-  | CandBegin => n + 1
-  | CandTraveling d => n - d
-  | CandLost => 0
-  end.
-
-(*
-  Correctness of system is a direct consequence of [election_variant = 0] is reachable
- *)
-Definition election_variant (st : election_state) :=
-  match st with
-  | VCandidates l => 2 * n + List.fold_left (fun m st => m + cand_state_value st) l 0
-  | VElected d => n - d
-  end.
+Definition handle_send qs st i (q : nat * bool) :=
+  if fst q then handle_next qs st ((i + 1) mod n) else (fst q - 1, false).
 
 Definition handle_election_state (qs: list (list message)) (st: election_state) :
   forall X, netE message X -> election_state :=
   fun X e =>
+  let m := (proj1_sig (Fin.to_nat (max_id wf))) in
+  let next := next_proc st in
   match e with
   | Send i to msg =>
-    match st, msg with
-    | VCandidates l, Candidate c =>
-      VCandidates (nth_map (fun i =>
-        match i with
-        | CandBegin => CandTraveling 0
-        | CandTraveling d => CandTraveling (S d)
-        | _ => CandLost
-        end)
-        l c)
-    | VCandidates l, Elected e => VElected 0
-    | VElected i, Elected e => VElected (S i)
-    | _, _ => VCandidates (List.repeat CandLost n)
+    let p := nth_map (fun _ => ProcWaiting) st.(s_procs) i in
+    let pe := nth_map (fun _ => ProcElected) st.(s_procs) i in
+    let q := if Nat.eqb i next then handle_send qs st i st.(s_queue) else st.(s_queue) in
+    match st.(s_progress), msg with
+    | MaxCandidate d, Candidate c =>
+      let progress := if Nat.eqb c ids[@max_id wf] then MaxCandidate (S d) else st.(s_progress) in
+      mk_election_state p progress q
+    | MaxElected d, Candidate c =>
+      mk_election_state p st.(s_progress) q
+    | MaxElected d, Elected e =>
+      mk_election_state pe (MaxElected (S d)) q
+    | MaxCandidate d, Elected e =>
+      mk_election_state pe (MaxElected 0) q
     end
-  | _ => st
+  | Recv i =>
+    let s := match hd_error (nth i qs []%list) with
+    | Some m => ProcProcessing m
+    | None => ProcWaiting
+    end in
+    mk_election_state (nth_map (fun _ => s) st.(s_procs) i) st.(s_progress)
+      (if Nat.eqb i next then handle_recv st.(s_queue) else st.(s_queue))
   end.
 
-(* Progress in Lef's sense is decreasing the variant, but here the variant decrease always *)
+#[local] Instance h : netE message ~~> state (list (list message) * election_state) := handler_netE handle_election_state.
+
+Lemma eq_dec_message : forall (m m' : message), {m = m'} + {m <> m'}.
+Proof.
+  intros. destruct (m), m'.
+  2, 3: right; intro; discriminate.
+  - destruct (Nat.eq_dec u u0).
+    + subst. auto.
+    + right. intro. now injection H.
+  - destruct (Nat.eq_dec u u0).
+    + subst. auto.
+    + right. intro. now injection H.
+Qed.
+
+(* Three components in the "moral" configuration: the code, the dynamic state, the logical state.
+The invariants relate these three components. *)
+
+(* Invariant for the Candidate messages *)
+Definition election_invariant_candidates
+  st qs :=
+  (* Well-formedness *)
+  let procs := st.(s_procs) in
+  let m := (proj1_sig (Fin.to_nat (max_id wf))) in
+  (forall i, count_occ eq_dec_message (concat (ext_mailbox qs st)) (Candidate i) <= 1) /\
+  (forall i j, In (Candidate i) (List.nth j (ext_mailbox qs st) []%list) -> exists k, i = ids[@k]) /\
+  forall i (Hi : (i < n)%nat),
+    match List.nth_error procs i with
+    | Some ProcBegin => ~ In (Candidate i) (concat (ext_mailbox qs st))
+    | _ =>
+      (* A losing candidate cannot travel beyond the process with the max id *)
+      (forall k, k <> m -> In (Candidate ids[@Fin.of_nat_lt Hi]) (List.nth k (ext_mailbox qs st) []%list) -> from_to ((i + 1) mod n) ((m + 1) mod n) k)
+    end.
+
+(* Invariant regarding the position in the mailbox of the current message of interest *)
+Definition election_invariant_msg_location
+  (st : election_state) (qs: list (list message)) (i: nat) (m: message) :=
+  snd st.(s_queue) = match List.nth i st.(s_procs) ProcBegin with ProcProcessing m => true | _ => false end /\
+  forall j k, List.nth_error (List.nth j (ext_mailbox qs st) []%list) k = Some m <-> j = i /\ k = fst st.(s_queue).
+
+(* Invariant regarding the max candidate *)
+Definition election_invariant_max
+  (st : election_state) (qs: list (list message)) :=
+  let m := (proj1_sig (Fin.to_nat (max_id wf))) in
+  let elected_progress := st.(s_progress) in
+  fst st.(s_queue) < n /\
+  match elected_progress with
+  | MaxCandidate d =>
+    (* The leader has not been elected yet *)
+    (forall c, ~In (Elected c) (concat (ext_mailbox qs st))) /\
+    {Hd : d <= n |
+      (* The message can only be in the mailbox at distance d from the max *)
+      (d <> 0 -> election_invariant_msg_location st qs ((m + d) mod n) (Candidate ids[@max_id wf])) /\
+      (d = 0 -> ~In (Candidate ids[@max_id wf]) (concat (ext_mailbox qs st)))
+    }
+  | MaxElected elected_progress =>
+    {He : elected_progress < n |
+      let e' := Fin.of_nat_lt He in
+      let j := (m + elected_progress + 1) mod n in
+      (* There are no (Candidate m) messages left *)
+      (forall k, ~ In (Candidate ids[@max_id wf]) (List.nth k (ext_mailbox qs st) []%list)) /\
+      (* There can only be one elected message *)
+      election_invariant_msg_location st qs j (Elected ids[@max_id wf]) /\
+      forall c k, c <> ids[@max_id wf] -> ~In (Elected c) (List.nth k (ext_mailbox qs st) []%list)
+    }
+  end.
+
+Definition election_state_invariant st qs :=
+  List.length st.(s_procs) = n /\
+  election_invariant_candidates st qs /\
+  election_invariant_max st qs.
+
+(* Ties the proc_states to the ctrees *)
+Definition election_src_invariant_candidate st i (t : ctree (netE message) B01 unit) :=
+  match st with
+  | ProcBegin => t ≅ proc i n
+  | ProcWaiting =>
+    (t ≅ proc_loop i ((i + 1) mod n))
+  | ProcProcessing m => t ≅ proc_handle_msg i ((i + 1) mod n) (Some m);; proc_loop i ((i + 1) mod n)
+  | ProcElected => t ≅ Ret tt \/ t ≅ stuckD
+  end.
+
+(* Links proc_states and election progress *)
+Definition election_src_invariant st (v : vec n (ctree (netE message) B01 unit)) :=
+  let m := proj1_sig (Fin.to_nat (max_id wf)) in
+  (forall i (Hi : i < n),
+    election_src_invariant_candidate (nth i st.(s_procs) ProcBegin) i v[@Fin.of_nat_lt Hi]) /\
+  match st.(s_progress) with
+  | MaxCandidate d =>
+    (d = 0 -> nth m st.(s_procs) ProcBegin = ProcBegin) /\
+    forall k, nth k st.(s_procs) ProcBegin <> ProcElected
+  | MaxElected d =>
+    forall i (Hi: i < n),
+    nth i st.(s_procs) ProcBegin <> ProcBegin /\
+    (from_to ((S m) mod n) ((m + d + 1) mod n) i <->
+      nth i st.(s_procs) ProcBegin = ProcElected)
+  end.
+
+Definition election_invariant v qs st := election_state_invariant st qs /\ election_src_invariant st v.
+Opaque election_invariant.
+
+Lemma election_elected_proc_states :
+  forall v qs st d,
+  election_invariant v qs st ->
+  st.(s_progress) = MaxElected d ->
+  forall i (Hi : i < n),
+  let m := proj1_sig (Fin.to_nat (max_id wf)) in
+  (from_to ((S m) mod n) ((m + d + 1) mod n) i /\
+    nth i st.(s_procs) ProcBegin = ProcElected) \/
+  ( ~from_to ((S m) mod n) ((m + d + 1) mod n) i /\
+    (nth i st.(s_procs) ProcBegin = ProcWaiting \/
+      exists m, nth i st.(s_procs) ProcBegin = ProcProcessing m)).
+Proof.
+  intros. destruct H as [_ ?]. destruct H as [_ ?]. rewrite H0 in H.
+  destruct (from_to_dec (S m mod n) ((m + d + 1) mod n) i).
+  - left. split; auto.
+    now apply H in f.
+  - right. split; auto.
+    apply H in Hi as [? ?]. apply not_iff_compat in H2. apply H2 in n0.
+    destruct (nth i (s_procs st) ProcBegin) eqn:?; eauto with exfalso.
+Qed.
+
+Lemma election_map_proc_state :
+  forall v qs st i (Hi : i < n), election_invariant v qs st ->
+    election_src_invariant_candidate (nth i st.(s_procs) ProcBegin) i v[@Fin.of_nat_lt Hi].
+Proof.
+  intros. destruct H as [_ ?]. destruct H as [? _]. apply H.
+Qed.
+
 (*
-  checking your mailbox and it's empty ~> hidden by interpretation
-  Relies on a «medium step» so to speak: «internal» steps are aggregated together with the next «visible» step.
-
-  Are they useful ~> ???
-
-  What have we proved in the end?
-
-  ctree E
-  L == Ldata
-  E X -> L -> L
-
-
-
-  handle h ∘ handle g
-
+  Correctness of system is a direct consequence of [election_variant = 0] is reached
  *)
-Theorem election_progress :
-  forall (sched : vec n (ctree (netE message) B01 unit) -> ctree (netE message) B01 unit)
-  (Hc : sched_correct sched) (Hf : sched_fair sched)
-  v qs st, election_invariant v qs st -> election_variant st > 0 -> ~is_stuck (sched v).
+Definition election_variant (st : election_state) : nat * (nat * nat) :=
+  match st.(s_progress) with
+  | MaxCandidate d => (n + n + 1 - d, (fst st.(s_queue), if snd st.(s_queue) then 0 else 1))
+  | MaxElected d => (n - d - 1, (fst st.(s_queue), if snd st.(s_queue) then 0 else 1))
+  end.
+
+Definition lt_election_variant := slexprod nat (nat * nat) Nat.lt (slexprod nat nat Nat.lt Nat.lt).
+
+Lemma election_variant_wf : well_founded lt_election_variant.
+Proof.
+  repeat apply wf_slexprod; apply lt_wf.
+Qed.
+
+Theorem election_does_progress :
+  forall (sched : vec n (ctree (netE message) B01 unit) -> ctree (netE message) B01 unit) next_id
+  (Hc : sched_correct sched next_id)
+  v qs st, election_invariant v qs st -> election_variant st <> (0, (0, 0)) ->
+  exists l T', trans l (sched v) T'.
+Proof.
+Admitted.
+
+Lemma in_not_nil : forall {A} (l : list A) a, List.In a l -> l <> []%list.
+Proof.
+  intros * ? ->. destruct H.
+Qed.
+
+Lemma nth_not_default : forall {A} (l : list A) n d, List.nth n l d <> d -> n < length l.
+Proof.
+  intros. revert l H. induction n0; intros.
+  - destruct l. cbn in H. contradiction. cbn. lia.
+  - destruct l. cbn in H. contradiction. cbn in H. apply IHn0 in H. cbn. lia.
+Qed.
+
+(* Messages that do not make the system progress are
+   non-maximal Candidate messages *)
+Lemma election_other_messages :
+  let m := proj1_sig (Fin.to_nat (max_id wf)) in
+  forall v qs st msg k,
+  election_invariant v qs st ->
+  k <> next_proc st ->
+  In msg (List.nth k (ext_mailbox qs st) []%list) ->
+  exists i, i <> max_id wf /\ msg = Candidate ids[@i].
 Proof.
   intros.
-  destruct H. destruct st.
-  - clear H0. cbn in H, H1. destruct H. destruct H0.
-    specialize (H1 (proj1_sig (Fin.to_nat (max_id wf))) (proj2_sig (Fin.to_nat (max_id wf)))).
-    destruct (nth (proj1_sig (Fin.to_nat (max_id wf))) l CandLost) eqn:?.
-    + cbn in H1. eapply sched_fair_not_stuck; auto. rewrite H1.
-      intro. eapply H3. etrans.
-    + cbn in H1. eapply sched_fair_not_stuck; auto. admit.
-    + auto.
+  destruct H as [? _]. destruct H as (? & ? & ?). destruct H3.
+  destruct (s_progress st) eqn:?.
+  - (* phase 1 *)
+    destruct H4 as (? & ? & ?).
+    assert (k < length (ext_mailbox qs st)).
+    { eapply nth_not_default. eapply in_not_nil. apply H1. }
+    destruct msg.
+    2: {
+      exfalso. apply (H4 u). apply in_concat. eexists. split; [| apply H1].
+      now apply nth_In.
+    }
+    destruct H2 as (_ & ? & _).
+    apply H2 in H1 as ?. destruct H6 as [? ->].
+    exists x0. split; auto. intro. subst.
+    destruct (nat_eqdec n0 0).
+    + apply a in e. apply e.
+      apply in_concat. eexists. split; [| apply H1].
+      now apply nth_In.
+    + apply a in n1. destruct n1 as [_ ?].
+      apply In_nth_error in H1 as []. apply H6 in H1 as [-> ->].
+      unfold next_proc, next_proc_and_msg in H0. rewrite Heqe in H0. contradiction.
+  - (* phase 2 *)
+    destruct H4 as (? & ? & ?).
+    assert (k < length (ext_mailbox qs st)).
+    { eapply nth_not_default. eapply in_not_nil. apply H1. }
+    destruct msg.
+    + destruct H2 as (_ & ? & _). apply H2 in H1 as ?. destruct H7 as [? ->].
+      exists x0. split; auto. intro. subst.
+      now apply H4 in H1.
+    + exfalso. destruct (nat_eqdec u ids[@max_id wf]). subst.
+      * destruct H5 as [ [_ ?] _]. red in H5.
+        apply In_nth_error in H1 as []. apply H5 in H1 as [-> ->].
+        unfold next_proc, next_proc_and_msg in H0. rewrite Heqe in H0. contradiction.
+      * now apply H5 in H1.
+Qed.
+
+Lemma election_processing_ext_mailbox :
+  forall v qs st i (Hi : i < n) msg,
+  election_invariant v qs st ->
+  nth i (s_procs st) ProcBegin = ProcProcessing msg ->
+  hd_error (nth i (ext_mailbox qs st) []%list) = Some msg.
+Proof.
+  intros.
+  destruct H as [(? & _ & _) [? _] ].
+  specialize (H1 i Hi). red in H1. rewrite H0 in H1.
+  change []%list with (ext_mailbox1 ([]%list, ProcBegin)).
+  unfold ext_mailbox. rewrite map_nth. unfold ext_mailbox1. Search combine nth.
+  rewrite combine_nth, H0. reflexivity. admit. (* TODO add qs length to invariant *)
+Admitted.
+
+Lemma hd_error_in : forall {A} (l : list A) a, hd_error l = Some a -> In a l.
+Proof.
+  intros. destruct l; [discriminate |].
+  inversion H. subst. now left.
+Qed.
+
+(* ktrans inversion lemmas for leader election processes *)
+
+Lemma ktrans_proc_loop_some_inv : forall i j t' qs qs' st st' m,
+  ktrans ((proc_loop i j), (qs, st)) (t', (qs', st')) ->
+  List.hd_error (List.nth i qs []%list) = Some m ->
+  t' ≅ proc_loop_handle_msg i j (Some m) /\
+  qs' = nth_map (fun _ => tl (List.nth i qs []%list)) qs i /\
+  st' = mk_election_state
+    (nth_map (fun _ => ProcProcessing m) st.(s_procs) i)
+    st.(s_progress)
+    (if i =? next_proc st then handle_recv (s_queue st) else s_queue st).
+Proof.
+  intros.
+  unfold proc_loop in H. rewrite unfold_iter in H.
+  rewrite bind_bind in H. setoid_rewrite bind_trigger in H.
+  apply ktrans_vis_inv in H as (? & ? & ? & ?).
+  cbn in H2. unfold execState in H2. cbn in H1, H2.
+  destruct (nth i qs []%list) eqn:?. { discriminate. }
+  inv H0.
+  inversion H2. cbn. intuition.
+  cbn in H. unfold proc_loop_handle_msg, proc_handle_msg.
+  rewrite H. upto_bind_eq. destruct x1 as [ [] | [] ]; reflexivity.
+Qed.
+
+Lemma ktrans_proc_loop_none_inv : forall i j t' qs qs' st st',
+  ktrans ((proc_loop i j), (qs, st)) (t', (qs', st')) ->
+  List.hd_error (List.nth i qs []%list) = None ->
+  t' ≅ Guard (proc_loop i j) /\
+  qs' = qs /\
+  st' = st.
+Proof.
+  intros.
+  unfold proc_loop in H. rewrite unfold_iter in H.
+  rewrite bind_bind in H. setoid_rewrite bind_trigger in H.
+  apply ktrans_vis_inv in H as (? & ? & ? & ?).
+  cbn in H2. unfold execState in H2. cbn in H1, H2.
+  destruct (nth i qs []%list) eqn:?. 2: discriminate.
+  cbn in H1, H2. inv H2. intuition.
+  rewrite H. cbn. rewrite bind_ret_l. now apply br_equ.
+Qed.
+
+(*
+Lemma ktrans_proc_handle_other_candidate_gt_inv : forall i j c t' v qs qs' st st'
+  (INV: election_invariant v qs st),
+  ktrans (proc_loop_handle_msg i j (Some (Candidate c)), (qs, st)) (t', (qs', st')) ->
+  c > i ->
+  i <> next_proc st ->
+  t' ≅ Guard (proc_loop i j) /\
+  qs' = nth_map (fun q => (q ++ [Candidate c])%list) qs j /\
+  st' = mk_election_state
+    (nth_map (fun _ => ProcWaiting) st.(s_procs) i)
+    st.(s_progress)
+    st.(s_queue).
+Proof.
+  intros.
+  unfold proc_loop_handle_msg, proc_handle_msg in H.
+  apply Nat.compare_gt_iff in H0. rewrite H0 in H.
+  rewrite bind_bind in H. setoid_rewrite bind_trigger in H.
+  apply ktrans_vis_inv in H as ([] & ? & _ & ?). rewrite bind_ret_l in H.
+  cbn in H2. unfold execState in H2. cbn in H2.
+  inversion H2.
+  apply Nat.eqb_neq in H1. rewrite !H1.
+  destruct (s_progress st) eqn:?.
+  - assert (In (Candidate c) (List.nth i (ext_mailbox qs st) []%list)).
+    {
+      apply hd_error_in. eapply election_processing_ext_mailbox; eauto.
+*)
+
+(* Stability of variant when an uninteresting process is scheduled *)
+Theorem election_cst_elected :
+  let m := proj1_sig (Fin.to_nat (max_id wf)) in
+  forall i (Hi : i <> 0 /\ i < n) v T st st' qs qs',
+  election_invariant v qs st ->
+  fst (election_variant st) = i ->
+  proj1_sig (Fin.to_nat (next_id v)) <> (m + (n - i)) mod n ->
+  ktrans (sched v, (qs, st)) (T, (qs', st')) -> election_variant st' = election_variant st.
+Proof.
+  intros.
+  destruct st as [? [] ].
+  { cbn in H0. destruct H as [(? & ? & ?) _]. cbn in H4. destruct H4 as (? & _ & []). lia. }
+  unshelve eapply election_does_progress in H as ?; eauto.
+  2: { cbn. cbn in H0. intro. inversion H3. lia. }
+  destruct H3 as (? & ? & ?).
+  eapply sched_correct_ktrans in H2 as ?; eauto. destruct H4 as (? & ? & ?). subs.
+  pose proof (election_elected_proc_states H eq_refl (proj2_sig (Fin.to_nat (next_id v)))).
+  apply election_map_proc_state with (Hi := proj2_sig (Fin.to_nat (next_id v))) in H as ?.
+  rewrite Fin.of_nat_to_nat_inv in H6.
+  destruct H5 as [ [_ ?] | [_ ?] ].
+  - (* ProcElected *)
+    rewrite H5 in H6. red in H6. destruct H6.
+    + rewrite H6 in H4. apply ktrans_ret in H4 as []. inversion H7. now subst.
+    + rewrite H6 in H4. apply ktrans_trans in H4 as [(? & ?) | (? & ? & ? & ?)]; inv_trans.
+  - destruct H5 as [? | [] ].
+    + (* ProcWaiting *)
+      rewrite H5 in H6. red in H6. rewrite H6 in H4.
+      destruct (List.hd_error (List.nth (proj1_sig (Fin.to_nat (next_id v))) qs []%list)) eqn:?.
+      * (* non-empty mailbox *)
+        apply ktrans_proc_loop_some_inv with (m := m0) in H4 as (? & -> & ->); auto.
+        cbn. f_equal. destruct (_ =? _) eqn:?; auto.
+        apply Nat.eqb_eq in Heqb. cbn in Heqb. cbn in H0. subst. rewrite Heqb in H1.
+        clear -H1 Hi. exfalso. apply H1. apply Nat.mod_wd; auto. lia.
+      * (* empty mailbox *)
+        now apply ktrans_proc_loop_none_inv in H4 as (? & -> & ->).
+    + (* ProcProcessing *)
+      rewrite H5 in H6. red in H6. rewrite H6 in H4.
+      eapply election_processing_ext_mailbox in H5; eauto. 2: apply (proj2_sig (Fin.to_nat (next_id v))).
+      apply hd_error_in in H5. eapply election_other_messages in H5; eauto.
+      2: { cbn in H0 |- *. intro. apply H1. rewrite H7. apply Nat.mod_wd; auto. lia. }
+      destruct H5 as (? & ? & ->).
 Abort.
 
 End Election.
